\section{Recursión}
\begin{frame}[fragile]
  \frametitle{Recursión}
  {\color{white}
    \begin{minted}[bgcolor=bg]{haskell}
  factorial :: Num a => a -> a
  factorial 0 = 1
  factorial n = n * factorial (n - 1)
    \end{minted}
  }
\end{frame}

\begin{frame}[fragile]
  \frametitle{Recursión}
  {\color{white}
    \begin{minted}[bgcolor=bg]{haskell}
  duplicar :: Num a => [a] -> [a]
  duplicar []     = []
  duplicar [x]    = [x*2]
  duplicar (x:xs) = (x*2):(duplicar xs)
    \end{minted}
  }
  {\color{white}
    \begin{minted}[bgcolor=bg]{haskell}
  duplicar :: Num a => [a] -> [a]
  duplicar = map ((*) 2)
    \end{minted}
  }
\end{frame}

\begin{frame}{Aclaraciones}

\end{frame}